#### This document describes the variables in the tidydata.txt dataset

* Activity = description of the activity being performed
* Subject = Subject carrying out the activity
* timeBodyAccelerometer-mean()-X = average of Body accelerometer time signal X - mean
* timeBodyAccelerometer-mean()-Y = average of Body accelerometer time signal Y - mean
* timeBodyAccelerometer-mean()-Z = average of Body accelerometer time signal Z - mean
* timeBodyAccelerometer-std()-X = average of Body accelerometer time signal X - std
* timeBodyAccelerometer-std()-Y = average of Body accelerometer time signal Y - std
* timeBodyAccelerometer-std()-Z = average of Body accelerometer time signal Z - std
* timeGravityAccelerometer-mean()-X = average of Gravity accelerometer time signal X - mean
* timeGravityAccelerometer-mean()-Y = average of Gravity accelerometer time signal Y - mean
* timeGravityAccelerometer-mean()-Z = average of Gravity accelerometer time signal Z - mean
* timeGravityAccelerometer-std()-X = average of Gravity accelerometer time signal X - std
* timeGravityAccelerometer-std()-Y = average of Gravity accelerometer time signal Y - std
* timeGravityAccelerometer-std()-Z = average of Gravity accelerometer time signal Z - std
* timeBodyAccelerometerJerk-mean()-X = average of Body accelerometer jerk time signal X - mean
* timeBodyAccelerometerJerk-mean()-Y = average of Body accelerometer jerk time signal Y - mean
* timeBodyAccelerometerJerk-mean()-Z = average of Body accelerometer jerk time signal Z - mean
* timeBodyAccelerometerJerk-std()-X = average of Body accelerometer jerk time signal X - std
* timeBodyAccelerometerJerk-std()-Y = average of Body accelerometer jerk time signal Y - std
* timeBodyAccelerometerJerk-std()-Z = average of Body accelerometer jerk time signal Z - std
* timeBodyGyroscope-mean()-X = average of Body gyroscope time signal X - mean
* timeBodyGyroscope-mean()-Y = average of Body gyroscope time signal Y - mean
* timeBodyGyroscope-mean()-Z = average of Body gyroscope time signal Z - mean
* timeBodyGyroscope-std()-X = average of Body gyroscope time signal X - std
* timeBodyGyroscope-std()-Y = average of Body gyroscope time signal Y - std
* timeBodyGyroscope-std()-Z = average of Body gyroscope time signal Z - std
* timeBodyGyroscopeJerk-mean()-X = average of Body gyroscope jerk time signal X - mean
* timeBodyGyroscopeJerk-mean()-Y = average of Body gyroscope jerk time signal Y - mean
* timeBodyGyroscopeJerk-mean()-Z = average of Body gyroscope jerk time signal Z - mean
* timeBodyGyroscopeJerk-std()-X = average of Body gyroscope jerk time signal X - std
* timeBodyGyroscopeJerk-std()-Y = average of Body gyroscope jerk time signal Y - std
* timeBodyGyroscopeJerk-std()-Z = average of Body gyroscope jerk time signal Z - std
* timeBodyAccelerometerMagnitude-mean() = average of Body accelerometer magnitude time signal - mean
* timeBodyAccelerometerMagnitude-std() = average of Body accelerometer magnitude time signal - std
* timeGravityAccelerometerMagnitude-mean() = average of Body gyroscope magnitude time signal - mean
* timeGravityAccelerometerMagnitude-std() = average of Body gyroscope magnitude time signal - std
* timeBodyAccelerometerJerkMagnitude-mean() = average of Body accelerometer jerk magnitude time signal - mean
* timeBodyAccelerometerJerkMagnitude-std() = average of Body accelerometer jerk magnitude time signal - std
* timeBodyGyroscopeMagnitude-mean() = average of Body gyroscope magnitude time signal - mean
* timeBodyGyroscopeMagnitude-std() = average of Body gyroscope magnitude time signal - std
* timeBodyGyroscopeJerkMagnitude-mean() = average of Body gyroscope jerk magnitude time signal - mean
* timeBodyGyroscopeJerkMagnitude-std() = average of Body gyroscope jerk magnitude time signal - std
* frequencyBodyAccelerometer-mean()-X = average of Body accelerometer frequency signal X - mean
* frequencyBodyAccelerometer-mean()-Y = average of Body accelerometer frequency signal Y - mean
* frequencyBodyAccelerometer-mean()-Z = average of Body accelerometer frequency signal Z - mean
* frequencyBodyAccelerometer-std()-X = average of Body accelerometer frequency signal X - std
* frequencyBodyAccelerometer-std()-Y = average of Body accelerometer frequency signal Y - std
* frequencyBodyAccelerometer-std()-Z = average of Body accelerometer frequency signal Z - std
* frequencyBodyAccelerometerJerk-mean()-X = average of Body accelerometer frequency jerk signal X - mean
* frequencyBodyAccelerometerJerk-mean()-Y = average of Body accelerometer frequency jerk signal Y - mean
* frequencyBodyAccelerometerJerk-mean()-Z = average of Body accelerometer frequency jerk signal Z - mean
* frequencyBodyAccelerometerJerk-std()-X = average of Body accelerometer frequency jerk signal X - std
* frequencyBodyAccelerometerJerk-std()-Y = average of Body accelerometer frequency jerk signal Y - std
* frequencyBodyAccelerometerJerk-std()-Z = average of Body accelerometer frequency jerk signal Z - std
* frequencyBodyGyroscope-mean()-X = average of Body gyroscope frequency signal X - mean
* frequencyBodyGyroscope-mean()-Y = average of Body gyroscope frequency signal Y - mean
* frequencyBodyGyroscope-mean()-Z = average of Body gyroscope frequency signal Z - mean
* frequencyBodyGyroscope-std()-X = average of Body gyroscope frequency signal X - std
* frequencyBodyGyroscope-std()-Y = average of Body gyroscope frequency signal Y - std
* frequencyBodyGyroscope-std()-Z = average of Body gyroscope frequency signal Z - std
* frequencyBodyAccelerometerMagnitude-mean() = average of Body accelerometer magnitude frequency signal - mean
* frequencyBodyAccelerometerMagnitude-std() = average of Body accelerometer magnitude frequency signal - std
* frequencyBodyAccelerometerJerkMagnitude-mean() = average of Body accelerometer jerk magnitude frequency signal - mean
* frequencyBodyAccelerometerJerkMagnitude-std() = average of Body accelerometer jerk magnitude frequency signal - std
* frequencyBodyGyroscopeMagnitude-mean() = average of Body gyroscope magnitude frequency signal - mean
* frequencyBodyGyroscopeMagnitude-std() = average of Body gyroscope magnitude frequency signal - std
* frequencyBodyGyroscopeJerkMagnitude-mean() = average of Body gyroscope jerk magnitude frequency signal - mean
* frequencyBodyGyroscopeJerkMagnitude-std() = average of Body gyroscope jerk magnitude frequency signal - std
